examples/sgx/Test.fst
@@ -8,6 +8,8 @@ open Ast
 	
 
  In the below example, we are using only stack (but not heap because bitmap for heap should be set by V)
+ The example is complicated by making callee access caller for parameters. Hence the bitmap is set by caller
+ before invoking the callee 
 
  main:
 
@@ -20,12 +22,13 @@ open Ast
 
   rbx := 1300uL
   sub rax rsp rbx  
+  rbx := 1200uL
   div rcx rax 64uL
-  mod rax rax 64uL
+  mod rdx rax 64uL
   add rbx rbx rcx
   load rcx rbx
-  lsr rax 1uL rax
-  lor rax rcx rax
+  lsr rdx 1uL rdx
+  lor rax rcx rdx
   store rbx rax 
   rcx := 0
   rdx := 0
@@ -39,7 +42,7 @@ open Ast
  counter:
     push rbp
     rbp := rsp
-    add rbx rsp 2uL 
+    add rbx rsp 3uL 
     load rdx rbx
 
  L1: add rcx rcx 1
@@ -62,26 +65,27 @@ open Ast
 		 		(Push (1204uL, (Register "rbx")));
 				(Assign (1205uL, (Register "rbx"), (Constant 1300uL)));
 				(Sub (1206uL, (Register "rax"), (Register "rsp"),  (Register "rbx")));
-				(Div (1207uL, (Register "rcx"), (Register "rax"),  (Constant 64uL)));
-				(Mod (1208uL, (Register "rax"), (Register "rax"),  (Constant 64uL)));
-				(Add (1209uL, (Register "rbx"), (Register "rbx"),  (Register "rcx")));
-				(Load (1210uL, (Register "rcx"), 1uL, (Register "rbx")));
-				(Lsr (1211uL, (Register "rax"), (Constant 1uL), (Register "rax")));
-				(Lor (1212uL, (Register "rax"), (Register "rcx"), (Register "rax")));
-				(Store (1213uL, 1uL, (Register "rbx"), (Register "rax")));
-				(Assign (1214uL, (Register "rcx"), (Constant 0uL)));
-				(Assign (1215uL, (Register "rdx"), (Constant 0uL)));
-				(Assign (1216uL, (Register "r8"), (Constant 0uL)));
-				(Assign (1217uL, (Register "r9"), (Constant 0uL)));
-				(Call (1218uL, (Constant 1230uL)));
-		 		(Assign (1219uL, (Register "rsp"), (Register "rbp")));
-				(Pop (1220uL, (Register "rbp")));
-				(Return 1221uL)	
+				(Assign (1207uL, (Register "rbx"), (Constant 1200uL)));
+				(Div (1208uL, (Register "rcx"), (Register "rax"),  (Constant 64uL)));
+				(Mod (1209uL, (Register "rdx"), (Register "rax"),  (Constant 64uL)));
+				(Add (1210uL, (Register "rbx"), (Register "rbx"),  (Register "rcx")));
+				(Load (1211uL, (Register "rcx"), 1uL, (Register "rbx")));
+				(Lsr (1212uL, (Register "rdx"), (Constant 1uL), (Register "rdx")));
+				(Lor (1213uL, (Register "rax"), (Register "rcx"), (Register "rdx")));
+				(Store (1214uL, 1uL, (Register "rbx"), (Register "rax")));
+				(Assign (1215uL, (Register "rcx"), (Constant 0uL)));
+				(Assign (1216uL, (Register "rdx"), (Constant 0uL)));
+				(Assign (1217uL, (Register "r8"), (Constant 0uL)));
+				(Assign (1218uL, (Register "r9"), (Constant 0uL)));
+				(Call (1219uL, (Constant 1230uL)));
+		 		(Assign (1220uL, (Register "rsp"), (Register "rbp")));
+				(Pop (1221uL, (Register "rbp")));
+				(Return 1222uL)	
 				]));
 		("counter", 
 		 Seq (1230uL, [(Push (1230uL, (Register "rbp")));
 				(Assign (1231uL, (Register "rbp"), (Register "rsp")));
-				(Add (1232uL, (Register "rbx"), (Register "rsp"),(Constant 2uL)));
+				(Add (1232uL, (Register "rbx"), (Register "rsp"),(Constant 3uL)));
 				(Load (1233uL, (Register "rdx"), 1uL, (Register "rbx")));
 				(Add (1234uL, (Register "rcx"), (Register "rcx"),(Constant 1uL)));
 				(Cmp (1235uL, (Register "flag"), (Register "rdx"),(Register "rcx")));
